@prefix rdf: <http://www.w3.org/1999/02/22-rdf-syntax-ns#> .
@prefix shadow-rdf: <http://www.daml.org/services/owl-s/1.2/generic/ObjectList.owl#> .
@prefix rdfs: <http://www.w3.org/2000/01/rdf-schema#> .
@prefix owl: <http://www.w3.org/2002/07/owl#> .
@prefix service: <http://www.daml.org/services/owl-s/1.2/Service.owl#> .
@prefix process: <http://www.daml.org/services/owl-s/1.2/Process.owl#> .
@prefix : <http://www.daml.org/services/owl-s/1.2/Grounding.owl#> .

<http://www.daml.org/services/owl-s/1.2/Grounding.owl>
    a owl:Ontology ;
    rdfs:comment """
    Upper-level OWL ontology for Groundings that employ WSDL.
    Part of the OWL-S ontology; see http://www.daml.org/services/.

    This version is intended for use with WSDL 1.1.  The OWL-S
    Coalition plans to produce a future version for use with WSDL 2.0,
    when it has been finalized (or nearly so).

    Note that other approaches to grounding may be accommodated
    within the OWL-S framework.  This is the only approach produced
    to date by the OWL-S Coalition.

    For notes on version history, see 
        http://www.daml.org/services/owl-s/1.2/status.html.    
  """ ;
    owl:imports <http://www.daml.org/services/owl-s/1.2/Process.owl> ;
    owl:versionInfo """
    $Id: Grounding.owl,v 1.38 2006/01/04 21:41:56 martin Exp $
  """ .

:AtomicProcessGrounding
    a owl:Class ;
    rdfs:comment """
    A class that relates elements of a OWL-S atomic process to a
    WSDL specification.

    Each instance of AtomicProcessGrounding must have exactly one
    value for owlsProcess. Rest of the AtomicProcessGrounding depends
    on the specifics of the grounding type. 
  """ ;
    rdfs:subClassOf [
        a owl:Restriction ;
        owl:cardinality "1"^^<http://www.w3.org/2001/XMLSchema#nonNegativeInteger> ;
        owl:onProperty :owlsProcess
    ] .

:DirectInputMessageMap
    a owl:Class ;
    rdfs:subClassOf :WsdlInputMessageMap, [
        a owl:Restriction ;
        owl:cardinality "1"^^<http://www.w3.org/2001/XMLSchema#nonNegativeInteger> ;
        owl:onProperty :owlsParameter
    ], [
        a owl:Restriction ;
        owl:cardinality "0"^^<http://www.w3.org/2001/XMLSchema#nonNegativeInteger> ;
        owl:onProperty :xsltTransformation
    ] ;
    owl:disjointWith :XSLTInputMessageMap .

:DirectOutputMessageMap
    a owl:Class ;
    rdfs:subClassOf :WsdlOutputMessageMap, [
        a owl:Restriction ;
        owl:cardinality "1"^^<http://www.w3.org/2001/XMLSchema#nonNegativeInteger> ;
        owl:onProperty :wsdlMessagePart
    ], [
        a owl:Restriction ;
        owl:cardinality "0"^^<http://www.w3.org/2001/XMLSchema#nonNegativeInteger> ;
        owl:onProperty :xsltTransformation
    ] ;
    owl:disjointWith :XSLTOutputMessageMap .

:Grounding
    a owl:Class ;
    rdfs:comment """
    A Grounding is just a collection of AtomicProcessGrounding
    instances, one for each atomic process in the process model.    
  """ ;
    rdfs:subClassOf service:ServiceGrounding .

:InputMessageMap
    a owl:Class ;
    rdfs:comment """
    A MessageMap that maps inputs to grounding specification
  """ ;
    rdfs:subClassOf :MessageMap, [
        a owl:Restriction ;
        owl:allValuesFrom process:Input ;
        owl:onProperty :owlsParameter
    ] .

:MessageMap
    a owl:Class ;
    rdfs:comment """
    A class used to map parameters in OWL-S to the parameters
    in the grounded operation. owlsParamater property is used
    to specify the OWL-S parameter. 
  """ .

:OutputMessageMap
    a owl:Class ;
    rdfs:comment """
    A MessageMap that maps outputs to grounding specification
  """ ;
    rdfs:subClassOf :MessageMap, [
        a owl:Restriction ;
        owl:allValuesFrom process:Output ;
        owl:onProperty :owlsParameter
    ] .

:WsdlAtomicProcessGrounding
    a owl:Class ;
    rdfs:comment """
    A class that relates elements of a OWL-S atomic process to a
    WSDL specification.
  """, """
    Each instance of WsdlAtomicProcessGrounding must have exactly one
    value for owlsProcess and exactly one for wsdlOperation, which sets up
    a one-to-one correspondence between an atomic process and a WSDL
    operation.

    In addition, for each message part of the relevant WSDL input message,
    there must be exactly one value of wsdlInput.  For each output of the
    atomic process, there must be exactly one value of wsdlOutput. These
    property instances show the correspondences between OWL-S
    inputs/outputs and WSDL message parts.  In addition, single values are
    recommended (but not required) for wsdlInputMessage and
    wsdlOutputMessage.

    Note that the value of wsdlOperation may or may not uniquely identify
    a particular WSDL port with which to interact.  If there are multiple
    such ports offering the specified operation, an OWL-S enactment engine
    is free to choose any of these ports.  If it is desired to further
    constrain the choice of ports, a WsdlAtomicProcessGrounding may do so
    by specifying any number of values for wsdlService and/or wsdlPort.
  """ ;
    rdfs:subClassOf :AtomicProcessGrounding, [
        a owl:Restriction ;
        owl:cardinality "1"^^<http://www.w3.org/2001/XMLSchema#nonNegativeInteger> ;
        owl:onProperty :wsdlOperation
    ] .

:WsdlGrounding
    a owl:Class ;
    rdfs:comment """
    WsdlGrounding is A Grounding that grounds every process to 
    a WSDL operation.    
  """ ;
    rdfs:subClassOf :Grounding, [
        a owl:Restriction ;
        owl:allValuesFrom :WsdlAtomicProcessGrounding ;
        owl:onProperty :hasAtomicProcessGrounding
    ] .

:WsdlInputMessageMap
    a owl:Class ;
    rdfs:comment """
	The purpose of a WsdlInputMessageMap is to show how to derive the WSDL
	input message parts from the OWL-S Parameter values. There should be
	one WsdlInputMessageMap for each WSDL input message part.
	
	There are two different kinds of input message maps:
	
	(1) DirectInputMessageMap - This is used when we have a 1-1 mapping between
	Inputs in the AtomicProcess and WSDL message parts. There are two cases:
	
	(a) The parameterType of the Input is an OWL class.  The OWL class is
	used as the message part type in the WSDL document.  (Note: for this
	case to be fully general, further work may be needed to establish
	conventions for serializing arbitrary OWL instances).
	
	(b) The parameterType is an XSD simple type, and the WSDL message part
	has the same type.
	
	(2) XSLTInputMessageMap - This is used when the the parameterType and
	the WSDL message part type is not the same. The WSDL type can be
	either simple or complex.  In this case, a WSDL message part can be
	derived from multiple Inputs.
  """ ;
    rdfs:subClassOf :InputMessageMap, :WsdlMessageMap, [
        a owl:Restriction ;
        owl:cardinality "1"^^<http://www.w3.org/2001/XMLSchema#nonNegativeInteger> ;
        owl:onProperty :wsdlMessagePart
    ] ;
    owl:unionOf (:DirectInputMessageMap
        :XSLTInputMessageMap
    ) .

:WsdlMessageMap
    a owl:Class ;
    rdfs:comment """
    MessageMap for WSDL inputs and outputs
  """ ;
    rdfs:subClassOf :MessageMap .

:WsdlOperationRef
    a owl:Class ;
    rdfs:comment """
    Restricting the cardinality of operation to one
  """, """
    Restricting the cardinality of portType to one
  """, """
    This class provides a unique specification of a WSDL operation.
    WSDL 1.1, on which this version of the grounding is based, does 
    not have a way to uniquely identify an operation with a single URI.  
    Uniqueness is achieved using a pair (portType, operation).
  """ ;
    rdfs:subClassOf [
        a owl:Restriction ;
        owl:cardinality "1"^^<http://www.w3.org/2001/XMLSchema#nonNegativeInteger> ;
        owl:onProperty :portType
    ], [
        a owl:Restriction ;
        owl:cardinality "1"^^<http://www.w3.org/2001/XMLSchema#nonNegativeInteger> ;
        owl:onProperty :operation
    ] .

:WsdlOutputMessageMap
    a owl:Class ;
    rdfs:comment """
	The purpose of WsdlOutputMessageMap is to show how to derive OWL-S
	Parameter values from the WSDL output message parts. There should be
	one WsdlOutputMessageMap for each Output of the corresponding
	AtomicProcess.
	
	There are two kinds of output message maps, similarly to input message maps.
	
	(1) DirectOutputMessageMap - This is used when we have a 1-1 mapping between
	WSDL message parts and Outputs in the Atomic Process. There are two cases:
	
	(a) The parameterType of the Output is an OWL class, and the OWL class
	is used as the message part type in the WSDL document.  (Note: for
	this case to be fully general, further work may be needed to establish
	conventions for serializing arbitrary OWL instances).
	
	(b) The parameterType is an XSD simple type, and the WSDL message part
	has the same type.
	
	(2) XSLTOutputMessageMap - This is used when the the parameterType and
	the WSDL message part type is not the same. The WSDL type can be
	either simple or complex.  In this case, an OWL Output can be derived
	from multiple WSDL message parts.  
  """ ;
    rdfs:subClassOf :OutputMessageMap, :WsdlMessageMap, [
        a owl:Restriction ;
        owl:cardinality "1"^^<http://www.w3.org/2001/XMLSchema#nonNegativeInteger> ;
        owl:onProperty :owlsParameter
    ] ;
    owl:unionOf (:DirectOutputMessageMap
        :XSLTOutputMessageMap
    ) .

:XSLTInputMessageMap
    a owl:Class ;
    rdfs:subClassOf :WsdlInputMessageMap, [
        a owl:Restriction ;
        owl:cardinality "0"^^<http://www.w3.org/2001/XMLSchema#nonNegativeInteger> ;
        owl:onProperty :owlsParameter
    ], [
        a owl:Restriction ;
        owl:cardinality "1"^^<http://www.w3.org/2001/XMLSchema#nonNegativeInteger> ;
        owl:onProperty :xsltTransformation
    ] .

:XSLTOutputMessageMap
    a owl:Class ;
    rdfs:subClassOf :WsdlOutputMessageMap, [
        a owl:Restriction ;
        owl:cardinality "0"^^<http://www.w3.org/2001/XMLSchema#nonNegativeInteger> ;
        owl:onProperty :wsdlMessagePart
    ], [
        a owl:Restriction ;
        owl:cardinality "1"^^<http://www.w3.org/2001/XMLSchema#nonNegativeInteger> ;
        owl:onProperty :xsltTransformation
    ] .

:hasAtomicProcessGrounding
    a owl:ObjectProperty ;
    rdfs:domain :Grounding ;
    rdfs:range :AtomicProcessGrounding .

:operation
    a owl:DatatypeProperty ;
    rdfs:domain :WsdlOperationRef ;
    rdfs:range <http://www.w3.org/2001/XMLSchema#anyURI> .

:owlsParameter
    a owl:ObjectProperty ;
    rdfs:comment """
    An input or output property of an atomic process.
  """ ;
    rdfs:domain :MessageMap ;
    rdfs:range process:Parameter .

:owlsProcess
    a owl:FunctionalProperty, owl:ObjectProperty ;
    rdfs:comment """
    The atomic process to which this grounding applies.
  """ ;
    rdfs:domain :AtomicProcessGrounding ;
    rdfs:range process:AtomicProcess .

:portType
    a owl:DatatypeProperty ;
    rdfs:domain :WsdlOperationRef ;
    rdfs:range <http://www.w3.org/2001/XMLSchema#anyURI> .

:wsdlDocument
    a owl:DatatypeProperty ;
    rdfs:comment """
    A URI indicating a WSDL document to
    which this grounding refers.  This isn't
    essential; primarily for convenience as documentation.
  """ ;
    rdfs:domain :WsdlAtomicProcessGrounding ;
    rdfs:range <http://www.w3.org/2001/XMLSchema#anyURI> .

:wsdlInput
    a owl:ObjectProperty ;
    rdfs:comment """
    There should be one instance of this property for each
    message part of the WSDL input message.
  """ ;
    rdfs:domain :WsdlAtomicProcessGrounding ;
    rdfs:range :WsdlInputMessageMap .

:wsdlInputMessage
    a owl:DatatypeProperty, owl:FunctionalProperty ;
    rdfs:comment """
    A URI for the WSDL input message element corresponding
    to the inputs of the atomic process.
  """ ;
    rdfs:domain :WsdlAtomicProcessGrounding ;
    rdfs:range <http://www.w3.org/2001/XMLSchema#anyURI> .

:wsdlMessagePart
    a owl:DatatypeProperty ;
    rdfs:comment """
    A URI for a WSDL message part element.
  """ ;
    rdfs:domain :WsdlMessageMap ;
    rdfs:range <http://www.w3.org/2001/XMLSchema#anyURI> .

:wsdlOperation
    a owl:ObjectProperty ;
    rdfs:comment """
    A WSDL operation to which the atomic process
    (referenced by owlsProcess) corresponds.
  """ ;
    rdfs:domain :WsdlAtomicProcessGrounding ;
    rdfs:range :WsdlOperationRef .

:wsdlOutput
    a owl:ObjectProperty ;
    rdfs:comment """
    There should be one instance of this property for each
    output of the atomic process.
  """ ;
    rdfs:domain :WsdlAtomicProcessGrounding ;
    rdfs:range :WsdlOutputMessageMap .

:wsdlOutputMessage
    a owl:DatatypeProperty, owl:FunctionalProperty ;
    rdfs:comment """
    A URI for the WSDL message element corresponding
    to the outputs of the atomic process.
  """ ;
    rdfs:domain :WsdlAtomicProcessGrounding ;
    rdfs:range <http://www.w3.org/2001/XMLSchema#anyURI> .

:wsdlPort
    a owl:DatatypeProperty ;
    rdfs:comment """
    A URI for a WSDL Port that provides the operation to which 
    this atomic process is grounded.
  """ ;
    rdfs:domain :WsdlAtomicProcessGrounding ;
    rdfs:range <http://www.w3.org/2001/XMLSchema#anyURI> .

:wsdlService
    a owl:DatatypeProperty ;
    rdfs:comment """
    A URI for a WSDL Service that provides the operation to which 
    this atomic process is grounded.
  """ ;
    rdfs:domain :WsdlAtomicProcessGrounding ;
    rdfs:range <http://www.w3.org/2001/XMLSchema#anyURI> .

:wsdlVersion
    a owl:DatatypeProperty, owl:FunctionalProperty ;
    rdfs:comment """
    A URI indicating the version of WSDL being used.
  """ ;
    rdfs:domain :WsdlAtomicProcessGrounding ;
    rdfs:range <http://www.w3.org/2001/XMLSchema#anyURI> .

:xsltTransformation
    a owl:DatatypeProperty ;
    rdfs:comment """
    XSLT Tranformation to transform OWL-S parameters (inputs and outputs) 
    to and from WSDL messages.  This property exists mainly for declaring
    a cardinality restriction, and should not be instantiated
    directly.  Instantiate xsltTransformationString or xsltTransformationURI.
    (Ranges are specified with the sub properties.)
  """ ;
    rdfs:domain :WsdlMessageMap .

:xsltTransformationString
    a owl:DatatypeProperty ;
    rdfs:comment """
    A string giving an XSLT Tranformation.
  """ ;
    rdfs:range <http://www.w3.org/2001/XMLSchema#string> ;
    rdfs:subPropertyOf :xsltTransformation .

:xsltTransformationURI
    a owl:DatatypeProperty ;
    rdfs:comment """
    A URI for an XSLT Tranformation.
  """ ;
    rdfs:range <http://www.w3.org/2001/XMLSchema#anyURI> ;
    rdfs:subPropertyOf :xsltTransformation .

<http://www.daml.org/services/owl-s/1.2/Process.owl>
    a owl:Ontology .

